Partial proof for get_identifier_ref (just declarative envs).

LambdaS5/coq/LjsRulesCorrectExpressions.v
@@ -47,6 +47,114 @@ Implicit Type jder : J.decl_env_record.
 Implicit Type jprops : J.object_properties_type.
 Implicit Type jlenv : J.lexical_env.
 
+(* TODO move *)
+Lemma env_record_related_lookup_lemma : forall BR jeptr ptr jst st obj,
+     state_invariant BR jst st ->
+     fact_js_env jeptr ptr \in BR ->
+     binds st ptr obj ->
+     exists jer,
+     binds jst jeptr jer /\
+     env_record_related BR jer obj.
+Proof.
+    introv Hinv Hbs Hbinds.
+    lets Hjindex : heaps_bisim_consistent_lnoghost_env (state_invariant_heaps_bisim_consistent Hinv) Hbs.
+    lets (jer&Hjbinds) : index_binds Hjindex.
+    lets Herel : heaps_bisim_consistent_bisim_env (state_invariant_heaps_bisim_consistent Hinv) Hbs Hbinds.
+        eassumption.
+    jauto.
+Qed.
+
+(* TODO move *)
+Definition js_object_coercible jv := jv <> J.value_prim J.prim_undef /\ jv <> J.value_prim J.prim_null.
+
+Inductive ref_base_type_related BR : J.ref_base_type -> L.value -> Prop :=
+| ref_base_type_related_undefined : 
+    ref_base_type_related BR (J.ref_base_type_value (J.value_prim J.prim_undef)) L.value_null
+| ref_base_type_related_value : forall jv v,
+    js_object_coercible jv ->
+    value_related BR jv v ->
+    ref_base_type_related BR (J.ref_base_type_value jv) v
+| ref_base_type_related_env_loc : forall jeptr ptr,
+    fact_js_env jeptr ptr \in BR ->
+    ref_base_type_related BR (J.ref_base_type_env_loc jeptr) (L.value_object ptr).
+
+Hint Constructors ref_base_type_related : js_ljs.
+
+Hint Extern 5 (_ < _) => math : js_ljs.
+
+Lemma stx_eq_string_eq_lemma : forall s1 s2,
+    L.stx_eq (L.value_string s1) (L.value_string s2) = (s1 = s2).
+Proof.
+    introv. rew_logic. splits; introv Hx. {
+       inverts Hx. reflexivity.
+    } {
+       substs. eauto_js.
+    }
+Qed.
+
+Lemma decl_env_record_vars_related_index_lemma : forall BR jx x s,
+    decl_env_record_vars_related BR jx x ->
+    index jx s = index x s.
+Proof.
+    introv Hder.
+    specializes Hder s.
+    destruct Hder as [(Hder1&Hder2)|(?&?&?&Hder1&Hder2&Hder3)]. {
+        apply prop_eq_False_back in Hder1.
+        apply prop_eq_False_back in Hder2.
+        rewrite Hder1. rewrite Hder2. reflexivity.
+    } {
+        apply index_binds_inv in Hder1.
+        apply index_binds_inv in Hder2.
+        rew_logic; split; auto. 
+    }
+Qed.
+
+Lemma red_spec_lexical_env_get_identifier_ref_lemma : forall k BR jst jc c st st' r v s b v1 jlenv,
+    L.red_exprh k c st
+        (L.expr_app_2 LjsInitEnv.privEnvGetId [v; L.value_string s; v1]) (L.out_ter st' r) ->
+    state_invariant BR jst st ->
+    lexical_env_related BR jlenv v -> 
+    exists k' c' v' jrbt jst' st'' BR',
+    k' < k /\
+    BR \c BR' /\
+    state_invariant BR' jst' st'' /\
+    L.red_exprh k' c' st'' (L.expr_app_2 v1 [v']) (L.out_ter st' r) /\
+    J.red_spec jst jc (J.spec_lexical_env_get_identifier_ref jlenv s b) 
+        (J.specret_val jst' (J.ref_intro jrbt s b)) /\
+    ref_base_type_related BR' jrbt v'.
+Proof.
+    intro k.
+    induction_wf IH : lt_wf k.
+    introv Hlred Hinv Hlrel.
+    inverts red_exprh Hlred.
+    ljs_apply.
+    inverts Hlrel as Hlrel1 Hlrel2 Hlrel3. {
+        repeat ljs_autoforward.
+        jauto_js. 
+    }
+    repeat ljs_autoforward.
+    forwards (jer&Hjbinds&Herel) : env_record_related_lookup_lemma Hinv Hlrel1. eassumption.
+    inverts Herel as Herel. {
+        inverts Herel.
+        unfolds L.object_class.
+        cases_decide as Heq; rewrite stx_eq_string_eq_lemma in Heq; tryfalse.
+        repeat ljs_autoforward.
+        cases_decide as Hidx; repeat ljs_autoforward. { (* var found *)
+            erewrite <- decl_env_record_vars_related_index_lemma in Hidx by eassumption.
+            jauto_js 8.
+        } { (* not found *)
+            erewrite <- decl_env_record_vars_related_index_lemma in Hidx by eassumption.
+            rewrite <- decl_env_record_indom_to_libbag in Hidx. (* TODO can be removed somehow? *)
+            lets Hp : state_invariant_ctx_parent_ok Hinv Hlrel2.
+            destruct_hyp Hp. repeat binds_determine.
+            specializes IH ___; try eassumption. math.
+            destruct_hyp IH. jauto_js 8. 
+        }
+    } {
+        skip. (* TODO object environments *)
+    }
+Qed.
+
 (* Expressions *)
 
 (** *** Functions *)
@@ -564,23 +672,6 @@ Proof.
         inverts Hvrel; tryfalse. apply Hd.
         simpl. cases_if. eauto_js.
     }
-Qed.
-
-(* TODO move *)
-Lemma env_record_related_lookup_lemma : forall BR jeptr ptr jst st obj,
-     state_invariant BR jst st ->
-     fact_js_env jeptr ptr \in BR ->
-     binds st ptr obj ->
-     exists jer,
-     binds jst jeptr jer /\
-     env_record_related BR jer obj.
-Proof.
-    introv Hinv Hbs Hbinds.
-    lets Hjindex : heaps_bisim_consistent_lnoghost_env (state_invariant_heaps_bisim_consistent Hinv) Hbs.
-    lets (jer&Hjbinds) : index_binds Hjindex.
-    lets Herel : heaps_bisim_consistent_bisim_env (state_invariant_heaps_bisim_consistent Hinv) Hbs Hbinds.
-        eassumption.
-    jauto.
 Qed.
 
 Lemma implicit_this_lemma : forall BR k jst jc c st st' r jle jeptr v,
